verify/Compute.v
@@ -15,24 +15,15 @@ From BusyCoq Require Import Helper.
 From BusyCoq Require Import TM.
 Set Default Goal Selector "!".
 
-Definition ctape (S : Type) : Type := list S * S * list S.
+Module Compute (Ctx : Ctx).
+  Export Ctx.
+  Local Module TMs := TMs Ctx. Export TMs.
 
-Section TMs.
-  Context {Q Sym : Type}.
-  Variable q0 : Q.
-  Variable s0 : Sym.
-  Variable tm : TM Q Sym.
+(** During computation, a tape is represented similarly to [tape], but
+    with finite lists at each side, implicitly completed with [s0]. *)
+Definition ctape : Type := list Sym * Sym * list Sym.
 
-  Variable eqb_sym : Sym -> Sym -> bool.
-  Variable eqb_sym_spec : forall a b, reflect (a = b) (eqb_sym a b).
-
-  Variable eqb_q : Q -> Q -> bool.
-  Variable eqb_q_spec : forall a b, reflect (a = b) (eqb_q a b).
-
-  Notation tape := (tape Sym).
-  Notation ctape := (ctape Sym).
-  Notation c0 := (c0 q0 s0).
-
+(** Lifting [ctape] into the corresponding [tape]. *)
 Fixpoint lift_side (xs : list Sym) : Stream Sym :=
   match xs with
   | [] => const s0
@@ -45,6 +36,7 @@ Definition lift_tape (t : ctape) : tape :=
 Definition lift (c : Q * ctape) : Q * tape :=
   match c with (q, t) => (q, lift_tape t) end.
 
+(** Deciding whether two [ctape]s correspond to the same [tape]. *)
 Fixpoint empty_side (xs : list Sym) : bool :=
   match xs with
   | x :: xs => eqb_sym x s0 && empty_side xs
@@ -124,6 +116,7 @@ Proof.
   intros [H1 H2]. congruence.
 Qed.
 
+(** Movement on [ctape]s. *)
 Definition left (t : ctape) : ctape :=
   match t with
   | ([], s, r) => ([], s0, s :: r)
@@ -149,7 +142,8 @@ Proof.
   intros [[l s] [| s' r]]; reflexivity.
 Qed.
 
-Definition cstep (c : Q * ctape) : option (Q * ctape) :=
+(** Computable semantics of Turing machines. *)
+Definition cstep (tm : TM) (c : Q * ctape) : option (Q * ctape) :=
   match c with
   | q; l {{s}} r =>
     match tm (q, s) with
@@ -159,56 +153,55 @@ Definition cstep (c : Q * ctape) : option (Q * ctape) :=
     end
   end.
 
-Lemma cstep_halting : forall c,
-  cstep c = None -> halting tm (lift c).
+Lemma cstep_halting : forall tm c,
+  cstep tm c = None -> halting tm (lift c).
 Proof.
-  intros [q [[l s] r]] H. unfold halting.
+  introv H. destruct c as [q [[l s] r]]. unfold halting.
   simpl. simpl in H.
   destruct (tm (q; s)) as [[[s' []] q'] |]; try discriminate.
   reflexivity.
 Qed.
 
-Lemma cstep_some : forall c c',
-  cstep c = Some c' ->
+Lemma cstep_some : forall tm c c',
+  cstep tm c = Some c' ->
   lift c -[ tm ]-> lift c'.
 Proof.
-  introv H.
-  destruct c as [q [[l s] r]].
+  introv H. destruct c as [q [[l s] r]].
   simpl. simpl in H.
   destruct (tm (q; s)) as [[[s' []] q1] |] eqn:E; inverts H as; simpl.
   - rewrite lift_left. apply step_left. assumption.
   - rewrite lift_right. apply step_right. assumption.
 Qed.
 
-Fixpoint cmultistep (n : nat) (c : Q * ctape) : option (Q * ctape) :=
+Fixpoint cmultistep (tm : TM) (n : nat) (c : Q * ctape) : option (Q * ctape) :=
   match n with
   | 0 => Some c
   | S n' =>
-    match cstep c with
-    | Some c' => cmultistep n' c'
+    match cstep tm c with
+    | Some c' => cmultistep tm n' c'
     | None => None
     end
   end.
 
-Lemma cmultistep_some : forall n c c',
-  cmultistep n c = Some c' ->
+Lemma cmultistep_some : forall tm n c c',
+  cmultistep tm n c = Some c' ->
   lift c -[ tm ]->* n / lift c'.
 Proof.
   induction n; introv H; simpl in H.
   - inverts H. apply multistep_0.
-  - destruct (cstep c) as [c1 |] eqn:E.
+  - destruct (cstep tm c) as [c1 |] eqn:E.
     + apply IHn in H. apply cstep_some in E.
       eapply multistep_S; eassumption.
     + discriminate.
 Qed.
 
-Lemma cmultistep_halts_in : forall n c,
-  cmultistep n c = None ->
+Lemma cmultistep_halts_in : forall tm n c,
+  cmultistep tm n c = None ->
   exists n', n' < n /\ halts_in tm (lift c) n'.
 Proof.
   induction n; introv H.
   - discriminate.
-  - simpl in H. destruct (cstep c) as [c1 |] eqn:E.
+  - simpl in H. destruct (cstep tm c) as [c1 |] eqn:E.
     + apply IHn in H. apply cstep_some in E.
       destruct H as [n' [Hlt [ch [Hrun Hhalting]]]].
       exists (S n'). split.
@@ -223,8 +216,8 @@ Proof.
         ** assumption.
 Qed.
 
-Corollary cmultistep_halts : forall n c,
-  cmultistep n c = None ->
+Corollary cmultistep_halts : forall tm n c,
+  cmultistep tm n c = None ->
   halts tm (lift c).
 Proof.
   introv H.
@@ -233,12 +226,10 @@ Proof.
   exists n'. exact H.
 Qed.
 
+(** The starting configuration. *)
 Definition starting : Q * ctape := q0; [] {{s0}} [].
 
 Lemma lift_starting : lift starting = c0.
 Proof. reflexivity. Qed.
 
-End TMs.
-
-Arguments left : simpl never.
-Arguments right : simpl never.
+End Compute.
