verify/Extraction.v
@@ -1,0 +1,51 @@
+(** * Extraction to OCaml *)
+
+Set Warnings "-notation-overriden,-parsing,-deprecated-hint-without-locality".
+From Coq Require Extraction.
+Require Import ExtrOcamlBasic.
+Require Import ExtrOcamlIntConv.
+From BusyCoq Require Import Helper.
+From BusyCoq Require Import TM.
+From BusyCoq Require Import Cyclers.
+
+Inductive state := A | B | C | D | E.
+Inductive sym := S0 | S1.
+
+Module Ctx <: Ctx.
+  Definition Q := state.
+  Definition Sym := sym.
+  Definition q0 := A.
+  Definition s0 := S0.
+
+  Definition eqb_q (a b : Q) :=
+    match a, b with
+    | A, A => true
+    | B, B => true
+    | C, C => true
+    | D, D => true
+    | E, E => true
+    | _, _ => false
+    end.
+
+  Lemma eqb_q_spec : forall a b, reflect (a = b) (eqb_q a b).
+  Proof.
+    intros [] []; constructor; (reflexivity || discriminate).
+  Qed.
+
+  Definition eqb_sym (a b : Sym) :=
+    match a, b with
+    | S0, S0 => true
+    | S1, S1 => true
+    | _, _ => false
+    end.
+
+  Lemma eqb_sym_spec : forall a b, reflect (a = b) (eqb_sym a b).
+  Proof.
+    intros [] []; constructor; (reflexivity || discriminate).
+  Qed.
+End Ctx.
+
+Module Extraction := Cyclers Ctx.
+
+Extraction Language OCaml.
+Extraction "cyclers.ml" Extraction.verify_cycler nat_of_int.
